src/Lean/Meta/Tactic/Simp/BuiltinSimprocs/BitVec.lean
@@ -168,6 +168,8 @@ builtin_dsimproc [simp, seval] reduceGetMsb (getMsbD _ _) := reduceGetBit ``getM
 builtin_dsimproc [simp, seval] reduceClz (clz _) := reduceUnary ``BitVec.clz 2 BitVec.clz
 /-- Simplification procedure for `cpop` (population count) on `BitVec`. -/
 builtin_dsimproc [simp, seval] reduceCpop (cpop _) := reduceUnary ``BitVec.cpop 2 BitVec.cpop
+/-- Simplification procedure for `sqrt` (population count) on `BitVec`. -/
+builtin_dsimproc [simp, seval] reduceSqrt (sqrt _) := reduceUnary ``BitVec.sqrt 2 BitVec.sqrt
 
 /-- Simplification procedure for `getElem`  on `BitVec`. -/
 builtin_dsimproc [simp, seval] reduceGetElem ((_ : BitVec _)[_]) := fun e => do
