src/Std/Tactic/BVDecide/Bitblast/BVExpr/Circuit/Impl/Expr.lean
@@ -18,6 +18,7 @@ public import Std.Tactic.BVDecide.Bitblast.BVExpr.Circuit.Impl.Operations.Umod
 public import Std.Tactic.BVDecide.Bitblast.BVExpr.Circuit.Impl.Operations.Reverse
 public import Std.Tactic.BVDecide.Bitblast.BVExpr.Circuit.Impl.Operations.Clz
 public import Std.Tactic.BVDecide.Bitblast.BVExpr.Circuit.Impl.Operations.Cpop
+public import Std.Tactic.BVDecide.Bitblast.BVExpr.Circuit.Impl.Operations.Sqrt
 import Init.Data.Nat.Linear
 import Init.Omega
 
@@ -239,6 +240,7 @@ where
           apply AIG.LawfulVecOperator.le_size_of_le_aig_size (f := bitblast.blastCpop)
           omega
         ⟨⟨res, this⟩, cache.cast (AIG.LawfulVecOperator.le_size (f := bitblast.blastCpop) ..)⟩
+      | .sqrt => sorry
     | .append lhs rhs h =>
       let ⟨⟨⟨aig, lhs⟩, hlaig⟩, cache⟩ := goCache aig lhs cache
       let ⟨⟨⟨aig, rhs⟩, hraig⟩, cache⟩ := goCache aig rhs cache
@@ -355,6 +357,7 @@ theorem go_decl_eq (aig : AIG BVBit) (expr : BVExpr w) (cache : Cache aig) :
       rw [goCache_decl_eq]
       have := (goCache aig expr cache).result.property
       exact Nat.lt_of_lt_of_le h1 this
+    | .sqrt => sorry
   next lhsExpr rhsExpr h =>
     have hl := (goCache aig lhsExpr cache).result.property
     have hr := (goCache (goCache aig lhsExpr cache).1.1.aig rhsExpr (goCache aig lhsExpr cache).cache).result.property
