src/Std/Tactic/BVDecide/Reflect.lean
@@ -130,6 +130,10 @@ theorem cpop_congr (w : Nat) (x x' : BitVec w) (h : x = x') :
     BitVec.cpop x' = BitVec.cpop x := by
   simp [*]
 
+theorem sqrt_congr (w : Nat) (x x' : BitVec w) (h : x = x') :
+    BitVec.cpop x' = BitVec.cpop x := by
+  simp [*]
+
 end BitVec
 
 namespace Bool
